tmp/obj/Debug/net8.0/Clover_abs.AssemblyInfo.cs
@@ -13,7 +13,7 @@ using System.Reflection;
 [assembly: System.Reflection.AssemblyCompanyAttribute("Clover_abs")]
 [assembly: System.Reflection.AssemblyConfigurationAttribute("Debug")]
 [assembly: System.Reflection.AssemblyFileVersionAttribute("1.0.0.0")]
-[assembly: System.Reflection.AssemblyInformationalVersionAttribute("1.0.0+0dd9e1211847fbcc3fd07a3c727791bed1f77bf1")]
+[assembly: System.Reflection.AssemblyInformationalVersionAttribute("1.0.0+88bfbeb649967246ebb472617da27d50bee8c7d9")]
 [assembly: System.Reflection.AssemblyProductAttribute("Clover_abs")]
 [assembly: System.Reflection.AssemblyTitleAttribute("Clover_abs")]
 [assembly: System.Reflection.AssemblyVersionAttribute("1.0.0.0")]
